nola/examples/rust_halt/verify/mutlist.v
@@ -1,0 +1,113 @@
+(** * Singly linked list over a mutable reference *)
+
+From nola.examples.rust_halt Require Export rec mod sum prod mutref verify.util.
+
+Section mutlist.
+  Context `{!rust_haltGS CON Σ, !rust_haltC CON, !rust_haltJ CON JUDG Σ,
+    !Csem CON JUDG Σ, !Jsem JUDG (iProp Σ), !rust_haltCS CON JUDG Σ,
+    !rust_haltJS CON JUDG Σ}.
+
+  (** [ty_mutlist_gen]: Generator of the [mutlist] type *)
+  Definition ty_mutlist_gen' {X} (α : lft) (T : ty CON Σ X)
+    (Self : ty CON Σ (binₓ X)) : ty CON Σ (unitₓ +ₓ X *'ₓ binₓ X *'ₓ binₓ X) :=
+    ty_sum ty_unit (ty_prod T (ty_mutref α Self)).
+  Definition ty_mutlist_gen {X} (α : lft) (T : ty CON Σ X)
+    (Self : ty CON Σ (binₓ X)) : ty CON Σ (binₓ X) :=
+    ty_mod (X:=unitₓ +ₓ X *'ₓ binₓ X *'ₓ binₓ X) (Y:=binₓ X)
+      (bin_unwrap (A:=X)) (ty_mutlist_gen' α T Self).
+  (** [ty_mutlist_gen] is productive *)
+  #[export] Instance ty_mutlist_gen_productive {α X T} :
+    Productive (@ty_mutlist_gen α X T).
+  Proof.
+    move=> k ???. apply: ty_mod_preserv. apply: ty_sum_preserv=>//.
+    apply ty_prod_preserv=>//. exact: ty_mutref_productive.
+  Qed.
+
+  (** [ty_mutlist]: List over a mutable reference, modeled as a binary tree *)
+  Definition ty_mutlist {X} (α : lft) (T : ty CON Σ X) : ty CON Σ (binₓ X) :=
+    ty_rec (ty_mutlist_gen α T).
+
+  (** [ty_mutlist] satisfies [Ty] *)
+  #[export] Instance ty_mutlist_ty `{!Ty (X:=X) T} {α} :
+    Ty (ty_mutlist α (X:=X) T).
+  Proof. exact _. Qed.
+
+  (** [ty_mutlist] satisfies [TyOp] *)
+  #[export] Instance ty_mutlist_ty_op
+    `(!Ty (X:=X) T, !TyOpLe T κ 0 d, !LftIncl κ α) :
+    TyOpAt (ty_mutlist α T) κ d.
+  Proof.
+    apply (ty_rec_ty_op (F:=ty_mutlist_gen α T) ᵖ[(T, 0)'])=>/=; [|exact _].
+    move=> ??[??]. apply: ty_mod_ty_op. apply: ty_sum_ty_op.
+    apply: ty_prod_ty_op. exact: ty_op_le.
+  Qed.
+
+  (** [ty_mutlist] preserves [Send] *)
+  #[export] Instance ty_mutlist_send `{!Send (X:=X) T} {α} :
+    Send (ty_mutlist α T).
+  Proof. exact _. Qed.
+  (** [ty_mutlist] preserves [Sync] *)
+  #[export] Instance ty_mutlist_sync `{!Sync (X:=X) T} {α} :
+    Sync (ty_mutlist α T).
+  Proof. exact _. Qed.
+
+  (** [Resol] over [ty_mutlist] *)
+  Definition post_mutlist {A} (post : A → Prop) (t : bin A) :=
+    match t with BinLeaf => True | BinNode a tl tr => post a ∧ tr = tl end.
+  #[export] Instance resol_mutlist
+    `(!Ty (X:=X) T, !TyOp T κ, !ResolAt (X:=X) T κ post d, !LftIncl κ α) :
+    ResolAt (ty_mutlist α T) κ (post_mutlist post) d.
+  Proof.
+    rewrite /ty_mutlist. setoid_rewrite (ty_rec_unfold (F:=ty_mutlist_gen _ _)).
+    eapply resol_post.
+    { apply @resol_mod, @resol_sum; [exact: _|].
+      apply @resol_prod; [exact: _|exact: resol_mutref]. }
+    move=>/= [|??]//=.
+  Qed.
+
+  (** Left spine of [bin] *)
+  Fixpoint bin_lefts {A} (t : bin A) : list A :=
+    match t with BinLeaf => [] | BinNode a tl _ => a :: bin_lefts tl end.
+  (** [Real] over [ty_mutlist] *)
+  #[export] Instance real_mutlist
+    `(!LftIncl κ α, !TyOp' X T κ, !RealLe (A:=A) T κ get 0 d) :
+    RealAt (ty_mutlist α T) κ (λ t, get <$> bin_lefts t) d.
+  Proof.
+    apply (ty_rec_real (F:=ty_mutlist_gen α T) ᵖ[(T, existT A get, 0)'])=>/=;
+      [|exact _]=> ??[??].
+    eapply real_eq.
+    { apply @real_mod. eapply (real_compose list_wrap).
+      apply @real_sum; [exact: _|].
+      apply @real_prod; [exact: real_le|exact: real_mutref]. }
+    move=>/= [|???]//=.
+  Qed.
+  #[export] Instance real_list_length `(!LftIncl κ α, !TyOp' X T κ) :
+    Real (ty_mutlist α (X:=X) T) κ (λ t, length (bin_lefts t)).
+  Proof.
+    move=> ?. eapply real_eq. { eapply (real_compose length). exact _. }
+    move=>/= ?. by rewrite length_map.
+  Qed.
+
+  (** Fold and unfold [ty_mutlist] *)
+  Lemma ty_mutlist_unfold {α X T} :
+    ty_mutlist (X:=X) α T ≡ ty_mutlist_gen α T (ty_mutlist (X:=X) α T).
+  Proof. exact ty_rec_unfold. Qed.
+  Lemma subty_mutlist_fold `{!Ty (X:=X) T} {α δ} :
+    ⊢ subty δ (ty_mutlist_gen' α T (ty_mutlist α T)) (ty_mutlist (X:=X) α T)
+        bin_wrap.
+  Proof.
+    erewrite subty_proper_fun.
+    { iApply subty_trans; [|by iApply subty_rec_fold].
+      iApply (subty_to_mod (T:=ty_mutlist_gen' _ T _))=> ?.
+      exact bin_unwrap_wrap. }
+    move=>/= [[]|?]//=.
+  Qed.
+  Lemma subty_mutlist_unfold `{!Ty (X:=X) T} {α δ} :
+    ⊢ subty δ (ty_mutlist (X:=X) α T) (ty_mutlist_gen' α T (ty_mutlist α T))
+        bin_unwrap.
+  Proof.
+    erewrite subty_proper_fun.
+    { iApply subty_trans; [by iApply subty_rec_unfold|]. iApply subty_of_mod. }
+    by case.
+  Qed.
+End mutlist.
