README.md
@@ -224,3 +224,5 @@ All the Coq code is in [`nola/`](nola/) and structured as follows:
           type),
         [`list_more`](nola/examples/rust_halt/verify/list.v) (More on the list
           type)
+      - [`mutlist`](nola/examples/rust_halt/verify/mutlist.v) (Singly linked
+          list over a mutable reference),
